proof/specs/XMSS_RFCAbs_RFCConc.ec
@@ -1,0 +1,3 @@
+require import XMSS_PRF.
+require XMSS_RFC_Abs.
+
